change the spec of serialized iterators to only cover a prefix of the underlying serialized list

src/cbor/pulse/raw/everparse/CBOR.Pulse.Raw.EverParse.Iterator.fst
@@ -1,4 +1,5 @@
 module CBOR.Pulse.Raw.EverParse.Iterator
+open CBOR.Spec.Util
 open CBOR.Pulse.Raw.Util
 open CBOR.Pulse.Raw.Iterator
 open Pulse.Lib.Slice open Pulse.Lib.Pervasives open Pulse.Lib.Trade
@@ -10,6 +11,7 @@ module R = Pulse.Lib.Reference
 module SZ = FStar.SizeT
 module Trade = Pulse.Lib.Trade.Util
 module LP = LowParse.Pulse.VCList
+module U64 = FStar.UInt64
 
 let cbor_raw_serialized_iterator_match
   (#elt_high: Type0)
@@ -20,7 +22,10 @@ let cbor_raw_serialized_iterator_match
   (c: cbor_raw_serialized_iterator)
   (l: list elt_high)
 : Tot slprop
-= exists* l' . LP.pts_to_serialized (LP.serialize_nlist (c.len) s) c.s #pm l' ** pure (l == l')
+= exists* l' . LP.pts_to_serialized (LP.serialize_nlist c.glen s) c.s #(pm *. c.p) l' ** pure (
+     U64.v c.len <= c.glen /\
+     l == fst (List.Tot.splitAt (U64.v c.len) l')
+  )
 
 ```pulse
 ghost
@@ -34,16 +39,20 @@ fn cbor_raw_serialized_iterator_unfold
   (l: list elt_high)
 requires
   cbor_raw_serialized_iterator_match s pm c l
-returns res: squash (List.Tot.length l == c.len)
-ensures
-  LP.pts_to_serialized (LP.serialize_nlist (c.len) s) c.s #pm l **
+ensures exists* l' .
+  LP.pts_to_serialized (LP.serialize_nlist (c.glen) s) c.s #(pm *. c.p) l' **
+  pure (
+    U64.v c.len <= c.glen /\
+    l == fst (List.Tot.splitAt (U64.v c.len) l')
+  ) **
   trade
-    (LP.pts_to_serialized (LP.serialize_nlist (c.len) s) c.s #pm l)
+    (LP.pts_to_serialized (LP.serialize_nlist (c.glen) s) c.s #(pm *. c.p) l')
     (cbor_raw_serialized_iterator_match s pm c l)
 {
   unfold (cbor_raw_serialized_iterator_match s pm c l);
+  with l' . assert (LP.pts_to_serialized (LP.serialize_nlist (c.glen) s) c.s #(pm *. c.p) l');
   ghost fn aux (_: unit)
-    requires (emp ** LP.pts_to_serialized (LP.serialize_nlist (c.len) s) c.s #pm l)
+    requires (emp ** LP.pts_to_serialized (LP.serialize_nlist (c.glen) s) c.s #(pm *. c.p) l')
     ensures (cbor_raw_serialized_iterator_match s pm c l)
   {
     fold (cbor_raw_serialized_iterator_match s pm c l)
@@ -55,31 +64,83 @@ ensures
 
 ```pulse
 ghost
-fn cbor_raw_serialized_iterator_fold
+fn cbor_raw_serialized_iterator_fold // this function cannot be used to truncate iterators since we want to preserve the list l.
   (#elt_high: Type0)
   (#k: LP.parser_kind)
   (#p: LP.parser k elt_high)
   (s: LP.serializer p { k.parser_kind_subkind == Some LP.ParserStrong })
   (pm: perm)
   (c: cbor_raw_serialized_iterator)
-  (l: LP.nlist (c.len) elt_high)
+  (l: LP.nlist (c.glen) elt_high)
 requires
-  LP.pts_to_serialized (LP.serialize_nlist (c.len) s) c.s #pm l
+  LP.pts_to_serialized (LP.serialize_nlist (c.glen) s) c.s #(pm *. c.p) l ** pure (
+    Ghost.reveal c.glen == U64.v c.len
+  )
 ensures
   cbor_raw_serialized_iterator_match s pm c l **
   trade
     (cbor_raw_serialized_iterator_match s pm c l)
-    (LP.pts_to_serialized (LP.serialize_nlist (c.len) s) c.s #pm l)
+    (LP.pts_to_serialized (LP.serialize_nlist (c.glen) s) c.s #(pm *. c.p) l)
 {
+  List.Tot.append_l_nil l;
+  list_splitAt_append_elim l [];
   fold (cbor_raw_serialized_iterator_match s pm c l);
   ghost fn aux (_: unit)
     requires (emp ** cbor_raw_serialized_iterator_match s pm c l)
-    ensures (LP.pts_to_serialized (LP.serialize_nlist (c.len) s) c.s #pm l)
+    ensures (LP.pts_to_serialized (LP.serialize_nlist (c.glen) s) c.s #(pm *. c.p) l)
   {
-    unfold (cbor_raw_serialized_iterator_match s pm c l)
+    unfold (cbor_raw_serialized_iterator_match s pm c l);
+    with l' . assert (LP.pts_to_serialized (LP.serialize_nlist (c.glen) s) c.s #(pm *. c.p) l');
+    List.Tot.append_l_nil l';
+    list_splitAt_append_elim l' [];
+    rewrite (LP.pts_to_serialized (LP.serialize_nlist (c.glen) s) c.s #(pm *. c.p) l')
+      as (LP.pts_to_serialized (LP.serialize_nlist (c.glen) s) c.s #(pm *. c.p) l)
   };
   Trade.intro _ _ _ aux;
   ()
+}
+```
+
+```pulse
+ghost
+fn cbor_raw_serialized_iterator_fold_with_perm
+  (#elt_high: Type0)
+  (#k: LP.parser_kind)
+  (#p: LP.parser k elt_high)
+  (s: LP.serializer p { k.parser_kind_subkind == Some LP.ParserStrong })
+  (glen: nat)
+  (sl: slice LP.byte)
+  (pm': perm)
+  (l': LP.nlist (glen) elt_high)
+  (c: cbor_raw_serialized_iterator)
+  (pm: perm)
+  (l: list elt_high)
+requires
+  LP.pts_to_serialized (LP.serialize_nlist (glen) s) sl #(pm') l' ** pure (
+    Ghost.reveal c.glen == glen /\
+    c.s == sl /\
+    U64.v c.len <= Ghost.reveal c.glen /\
+    l == fst (List.Tot.splitAt (U64.v c.len) l') /\
+    pm' == pm *. c.p +. pm *. c.p
+  )
+ensures
+  cbor_raw_serialized_iterator_match s pm c l **
+  trade
+    (cbor_raw_serialized_iterator_match s pm c l)
+    (LP.pts_to_serialized (LP.serialize_nlist (glen) s) sl #(pm') l')
+{
+  LP.pts_to_serialized_share (LP.serialize_nlist (glen) s) sl;
+  fold (cbor_raw_serialized_iterator_match s pm c l);
+  ghost fn aux (_: unit)
+  requires
+    LP.pts_to_serialized (LP.serialize_nlist (glen) s) sl #(pm' /. 2.0R) l' ** cbor_raw_serialized_iterator_match s pm c l
+  ensures
+    LP.pts_to_serialized (LP.serialize_nlist (glen) s) sl #(pm') l'
+  {
+    unfold (cbor_raw_serialized_iterator_match s pm c l);
+    LP.pts_to_serialized_gather (LP.serialize_nlist (glen) s) sl
+  };
+  Trade.intro _ _ _ aux
 }
 ```
 
@@ -96,20 +157,10 @@ fn cbor_raw_serialized_iterator_is_empty_equiv
 requires
   cbor_raw_serialized_iterator_match s pm c l
 ensures
-  cbor_raw_serialized_iterator_match s pm c l ** pure (Nil? l <==> S.len c.s == 0sz)
+  cbor_raw_serialized_iterator_match s pm c l ** pure (Nil? l <==> c.len == 0uL)
 {
   cbor_raw_serialized_iterator_unfold s pm c l;
-  LP.pts_to_serialized_elim_trade (LP.serialize_nlist (c.len) s) c.s;
-  S.pts_to_len c.s;
-  Trade.trans _ _ (cbor_raw_serialized_iterator_match s pm c l);
   Trade.elim _ _;
-  let b : bool = Ghost.reveal c.len = 0;
-  if (b) {
-    ()
-  } else {
-    LP.serialize_nlist_cons (c.len - 1) s (List.Tot.hd l) (List.Tot.tl l);
-    ()
-  }
 }
 ```
 
@@ -126,7 +177,7 @@ fn cbor_raw_serialized_iterator_is_empty
   (#l: Ghost.erased (list elt_high))
 {
   cbor_raw_serialized_iterator_is_empty_equiv s pm c l;
-  (S.len c.s = 0sz)
+  (c.len = 0uL)
 }
 ```
 
@@ -167,17 +218,18 @@ fn cbor_raw_serialized_iterator_next
   (#l: Ghost.erased (list elt_high))
 {
   cbor_raw_serialized_iterator_unfold s pm i l;
-  LP.nlist_cons_as_nondep_then s i.len i.s;
+  with l' . assert (LP.pts_to_serialized (LP.serialize_nlist i.glen s) i.s #(pm *. i.p) l');
+  LP.nlist_cons_as_nondep_then s i.glen i.s;
   Trade.trans _ _ (cbor_raw_serialized_iterator_match s pm i l);
-  let len' : Ghost.erased nat = i.len - 1;
-  let k' : Ghost.erased LP.parser_kind = LP.parse_nlist_kind len' k;
-  let p' : LP.parser k' (LP.nlist len' elt_high) = LP.parse_nlist len' p;
-  let s' : LP.serializer p' = LP.serialize_nlist len' s;
-  let v' : Ghost.erased (elt_high & LP.nlist len' elt_high) = (List.Tot.hd l, List.Tot.tl l);
+  let glen' : Ghost.erased nat = i.glen - 1;
+  let k' : Ghost.erased LP.parser_kind = LP.parse_nlist_kind glen' k;
+  let p' : LP.parser k' (LP.nlist glen' elt_high) = LP.parse_nlist glen' p;
+  let s' : LP.serializer p' = LP.serialize_nlist glen' s;
+  let v' : Ghost.erased (elt_high & LP.nlist glen' elt_high) = Ghost.hide (List.Tot.hd l', List.Tot.tl l');
   assert (LP.pts_to_serialized
     (LPC.serialize_nondep_then s s')
     i.s
-    #pm
+    #(pm *. i.p)
     v'
   );
   let sp = LowParse.Pulse.Combinators.split_nondep_then
@@ -189,8 +241,8 @@ fn cbor_raw_serialized_iterator_next
     i.s;
   match sp {
     Mktuple2 s1 s2 -> {
-      unfold (LPC.split_nondep_then_post s s' i.s pm v' sp);
-      unfold (LPC.split_nondep_then_post' s s' i.s pm v' s1 s2);
+      unfold (LPC.split_nondep_then_post s s' i.s (pm *. i.p) v' sp);
+      unfold (LPC.split_nondep_then_post' s s' i.s (pm *. i.p) v' s1 s2);
       Trade.trans _ _ (cbor_raw_serialized_iterator_match s pm i l);
       let res = phi s1;
       with pm' . assert (elt_match pm' res (fst v'));
@@ -200,10 +252,13 @@ fn cbor_raw_serialized_iterator_next
       Trade.trans (elt_match pm' res (List.Tot.hd l)) _ _;
       let i' : cbor_raw_serialized_iterator = {
         s = s2;
-        len = len';
+        p = i.p /. 2.0R;
+        len = U64.sub i.len 1uL;
+        glen = glen';
       };
       pi := CBOR_Raw_Iterator_Serialized i';
-      cbor_raw_serialized_iterator_fold s pm i' (List.Tot.tl l);
+      perm_half_mult pm i.p;
+      cbor_raw_serialized_iterator_fold_with_perm s glen' s2 (pm *. i.p) (List.Tot.tl l') i' pm (List.Tot.tl l);
       Trade.prod
         (elt_match _ res (List.Tot.hd l))
         _
