src/cbor/pulse/raw/CBOR.Pulse.Raw.Util.fst
@@ -34,3 +34,9 @@ let half_mul (a b: real) : Lemma
 let perm_mul_div (a b: perm) : Lemma
   (a `perm_mul` (b `perm_div` a) == b)
 = ()
+
+let perm_half_mult
+  (pm ip: perm)
+: Lemma
+  (pm *. (ip /. 2.0R) +. pm *. (ip /. 2.0R) == pm *. ip)
+= ()
